src/Crypto/HKDF/HMAC.dfy
@@ -6,14 +6,16 @@ module {:extern "HMAC"} HMAC {
   import opened StandardLibrary
   import opened UInt = StandardLibrary.UInt
 
-  // Hash length in octets (bytes), e.g. GetHashLength(SHA256) ==> 256 bits = 32 bytes ==> n = 32
-  function method GetHashLength(algorithm: HKDFAlgorithms): (n: int32)
-    ensures algorithm == HKDF_WITH_SHA_256 ==> n == 32
-    ensures algorithm == HKDF_WITH_SHA_384 ==> n == 48
+  datatype {:extern "Digests"} Digests = SHA_256 | SHA_384
+
+  // Hash length in octets (bytes), e.g. GetHashLength(SHA_256) ==> 256 bits = 32 bytes ==> n = 32
+  function method GetHashLength(digest: Digests): (n: int)
+    ensures digest == SHA_256 ==> n == 32
+    ensures digest == SHA_384 ==> n == 48
   {
-    match algorithm {
-      case HKDF_WITH_SHA_256 => 32
-      case HKDF_WITH_SHA_384 => 48
+    match digest {
+      case SHA_256 => 32
+      case SHA_384 => 48
     }
   }
 
@@ -22,17 +24,17 @@ module {:extern "HMAC"} HMAC {
     // These functions are used to model the extern state
     // https://github.com/dafny-lang/dafny/wiki/Modeling-External-State-Correctly
     function {:extern} getKey(): seq<uint8> reads this
-    function {:extern} getAlgorithm(): HKDFAlgorithms reads this
+    function {:extern} getDigest(): Digests reads this
     function {:extern} getInputSoFar(): seq<uint8> reads this
 
-    constructor {:extern} (algorithm: HKDFAlgorithms)
-      ensures this.getAlgorithm() == algorithm
+    constructor {:extern} (digest: Digests)
+      ensures this.getDigest() == digest
       ensures this.getInputSoFar() == []
 
     method {:extern "Init"} Init(key: seq<uint8>)
       modifies this
       ensures this.getKey() == key;
-      ensures this.getAlgorithm() == old(this.getAlgorithm())
+      ensures this.getDigest() == old(this.getDigest())
       ensures this.getInputSoFar() == []
 
     method {:extern "BlockUpdate"} Update(input: seq<uint8>)
@@ -40,15 +42,15 @@ module {:extern "HMAC"} HMAC {
       requires |input| < INT32_MAX_LIMIT
       modifies this
       ensures this.getInputSoFar() == old(this.getInputSoFar()) + input
-      ensures this.getAlgorithm() == old(this.getAlgorithm())
+      ensures this.getDigest() == old(this.getDigest())
       ensures this.getKey() == old(this.getKey())
 
     method {:extern "GetResult"} GetResult() returns (s: seq<uint8>)
       requires |this.getKey()| > 0
       modifies this
-      ensures |s| == GetHashLength(this.getAlgorithm()) as int
+      ensures |s| == GetHashLength(this.getDigest())
       ensures this.getInputSoFar() == []
-      ensures this.getAlgorithm() == old(this.getAlgorithm())
+      ensures this.getDigest() == old(this.getDigest())
       ensures this.getKey() == old(this.getKey())
   }
 }
